Checkpoint.

MQuinnEquiv.v
@@ -753,3 +753,52 @@ Proof.
   + apply fold_constants_com_sound.
   + apply optimize_0plus_com_sound.
 Qed.
+
+Fixpoint subst_aexp (i : id) (u : aexp) (a : aexp) : aexp :=
+  match a with
+  | ANum n =>
+      ANum n
+  | AId i' =>
+      if beq_id i i' then u else AId i'
+  | APlus a1 a2 =>
+      APlus (subst_aexp i u a1) (subst_aexp i u a2)
+  | AMinus a1 a2 =>
+      AMinus (subst_aexp i u a1) (subst_aexp i u a2)
+  | AMult a1 a2 =>
+      AMult (subst_aexp i u a1) (subst_aexp i u a2)
+  end.
+
+Example subst_aexp_ex :
+  subst_aexp X (APlus (ANum 42) (ANum 53))
+             (APlus (AId Y) (AId X))
+= (APlus (AId Y) (APlus (ANum 42) (ANum 53))).
+Proof. reflexivity. Qed.
+
+Definition subst_equiv_property := forall i1 i2 a1 a2,
+  cequiv (i1 ::= a1;; i2 ::= a2)
+         (i1 ::= a1;; i2 ::= subst_aexp i1 a1 a2).
+
+Theorem subst_inequiv :
+  ~ subst_equiv_property.
+Proof.
+  unfold subst_equiv_property. intros Contra.
+  remember (X ::= APlus (AId X) (ANum 1);;
+            Y ::= AId X)
+  as c1.
+  remember (X ::= APlus (AId X) (ANum 1);;
+            Y ::= APlus (AId X) (ANum 1))
+  as c2.
+  assert (cequiv c1 c2) by (subst; apply Contra).
+  remember (t_update (t_update empty_state X 1) Y 1) as st1.
+  remember (t_update (t_update empty_state X 1) Y 2) as st2.
+  assert (H1: c1 / empty_state \\ st1);
+  assert (H2: c2 / empty_state \\ st2);
+  try (subst;
+       apply E_Seq with (st' := (t_update empty_state X 1));
+       apply E_Ass; reflexivity).
+  apply H in H1.
+  assert (Hcontra: st1 = st2). {
+      apply (ceval_deterministic c2 empty_state); assumption. }
+  assert (Hcontra': st1 Y = st2 Y) by (rewrite Hcontra; reflexivity).
+  subst. inversion Hcontra'.
+Qed.
